\documentclass[10pt,a4paper]{article}
\usepackage[landscape]{geometry}
\usepackage{fullpage}
\usepackage{breqn}
\begin{document}
\footnotesize
\begin{dmath*}
Omega = \frac{1-alppha}{1-alppha+alppha\, epsilon}
\end{dmath*}
\begin{dmath*}
psi_n_ya = \frac{1+phi}{alppha+phi+\left(1-alppha\right)\, siggma}
\end{dmath*}
\begin{dmath*}
lambda = \frac{\left(1-thetta\right)\, \left(1-thetta\, betta\right)}{thetta}\, Omega_{t}
\end{dmath*}
\begin{dmath*}
kappa = lambda_{t}\, \left(siggma+\frac{alppha+phi}{1-alppha}\right)
\end{dmath*}
\begin{dmath}
% Equation 1
ppi_{t}=betta\, ppi_{t+1}+kappa_{t}\, \tilde{y}_{t}
\end{dmath}
\begin{dmath}
% Equation 2
\tilde{y}_{t}=\tilde{y}_{t+1}-\frac{1}{siggma}\, \left(i_{t}-ppi_{t+1}-r\_nat_{t}\right)
\end{dmath}
\begin{dmath}
% Equation 3
i_{t}=ppi_{t}\, phi\_pi+\tilde{y}_{t}\, phi\_y+nu_{t}
\end{dmath}
\begin{dmath}
% Equation 4
r\_nat_{t}=siggma\, psi\_n\_ya_{t}\, \left(a_{t+1}-a_{t}\right)
\end{dmath}
\begin{dmath}
% Equation 5
r\_real_{t}=i_{t}-ppi_{t+1}
\end{dmath}
\begin{dmath}
% Equation 6
y\_nat_{t}=psi\_n\_ya_{t}\, a_{t}
\end{dmath}
\begin{dmath}
% Equation 7
\tilde{y}_{t}=y_{t}-y\_nat_{t}
\end{dmath}
\begin{dmath}
% Equation 8
nu_{t}=rho\_nu\, nu_{t-1}+eps\_nu_{t}
\end{dmath}
\begin{dmath}
% Equation 9
a_{t}=rho\_a\, a_{t-1}+eps\_a_{t}
\end{dmath}
\begin{dmath}
% Equation 10
y_{t}=a_{t}+\left(1+alppha\right)\, n_{t}
\end{dmath}
\begin{dmath}
% Equation 11
i\_an_{t}=i_{t}\, 4
\end{dmath}
\begin{dmath}
% Equation 12
r\_nat\_an_{t}=r\_nat_{t}\, 4
\end{dmath}
\begin{dmath}
% Equation 13
r\_real\_an_{t}=r\_real_{t}\, 4
\end{dmath}
\begin{dmath}
% Equation 14
pi\_an_{t}=ppi_{t}\, 4
\end{dmath}
\begin{dmath}
% Equation 15
m\_cresc\_an_{t}=4\, \left(ppi_{t}+y_{t}-y_{t-1}-eta\, \left(i_{t}-i_{t-1}\right)\right)
\end{dmath}
\begin{dmath}
% Equation 16
m\_real_{t}=y_{t}-i_{t}\, eta
\end{dmath}
\end{document}
